src/common/block_proposer/block_signing_functions.dfy
@@ -9,27 +9,38 @@ module Block_Signing_Functions{
         data: T,
         domain: Domain
     ): Root
+
+
     
-    function method compute_attestation_signing_root_with_attestation_and_epoch(
+    // function method compute_attestation_signing_root_with_attestation_and_epoch(
+    //     attestation_data: AttestationData, 
+    //     attestation_epoch: Epoch
+    // ): Root
+    // {
+    //     var domain := compute_domain(DOMAIN_BEACON_ATTESTER, attestation_epoch);
+    //     compute_signing_root(attestation_data, domain)
+    // }
+
+    function method compute_attestation_signing_root(
         attestation_data: AttestationData, 
-        attestation_epoch: Epoch
+        fork_version: Version
     ): Root
     {
-        var domain := compute_domain(DOMAIN_BEACON_ATTESTER, attestation_epoch);
+        var domain := compute_domain_with_fork_version(DOMAIN_BEACON_ATTESTER, fork_version);
         compute_signing_root(attestation_data, domain)
     }
 
     function method compute_randao_reveal_signing_root(slot: Slot): Root
     {   
         var epoch := compute_epoch_at_slot(slot);
-        var domain := compute_domain(DOMAIN_RANDAO, epoch);
+        var domain := compute_domain_with_epoch(DOMAIN_RANDAO, epoch);
         compute_signing_root(epoch, domain)
     }
     
     function method compute_block_signing_root(block: BeaconBlock): Root
     {
         var epoch := compute_epoch_at_slot(block.slot);
-        var domain := compute_domain(DOMAIN_BEACON_PROPOSER, epoch);
+        var domain := compute_domain_with_epoch(DOMAIN_BEACON_PROPOSER, epoch);
         compute_signing_root(block, domain)
     }   
 
